lean/privacy/actions/info.lean
@@ -129,7 +129,7 @@ structure CreateSubchannelInfo (crypto: Crypto) (inp: CreateSubchannelInput) (m:
   m': Memory
   h_m': m' = (create_subchannel crypto inp m |> process_action crypto m).m
   r_ne_zero: inp.r ≠ 0
-  channel_exists: m .ChannelHashes [crypto.hash [inp.c, inp.addralice, inp.addrbob, inp.Kbob]] ≠ 0
+  channel_exists: m .ChannelHashes [crypto.hash [inp.c, inp.addralice, inp.addrbob]] ≠ 0
   prev_subchannel_exists: inp.k₁ = 0 ∨ m .SubchannelTokens [crypto.hash [inp.c, inp.k₀, inp.k₁ - 1], 0] ≠ 0
   old_token_was_zero: m .SubchannelTokens [inp.subchannel_id crypto, 0] = 0
   old_hash_was_zero: m .SubchannelHashes [inp.subchannel_hash crypto] = 0
@@ -194,7 +194,7 @@ structure CreateNoteInfo (crypto: Crypto) (inp: CreateNoteInput) (m: Memory) whe
   old_value_was_zero: m .Notes [inp.note_id crypto, 0] = 0
   prev_note_exists: inp.i₁ = 0 ∨ m .Notes [crypto.hash [inp.c crypto, inp.token, inp.i₀, inp.i₁ - 1], 0] ≠ 0
   i₀_lt_MAX_I₀: inp.i₀ < crypto.MAX_I₀
-  subchannel_exists : m .SubchannelHashes [crypto.hash [inp.c crypto, inp.addrbob, inp.Kbob, inp.token]] ≠ 0
+  subchannel_exists : m .SubchannelHashes [crypto.hash [inp.c crypto, inp.addrbob, inp.token]] ≠ 0
   memory_diff₀: m' .Notes [inp.note_id crypto, 0] = crypto.pack inp.r (inp.enc crypto)
   memory_diff₁: m' .OpenNoteToken [inp.note_id crypto] = if inp.r = 1 then inp.token else 0
 
@@ -234,12 +234,13 @@ def create_note_info
 structure CancelNoteInfo (crypto: Crypto) (inp: CancelNoteInput) (m: Memory) where
   m': Memory
   h_m': m' = (cancel_note crypto inp m |> process_action crypto m).m
-  subchannel_exists: m .SubchannelHashes [crypto.hash [inp.c, inp.addrbob, inp.Kbob crypto, inp.token]] ≠ 0
+  subchannel_exists: m .SubchannelHashes [crypto.hash [inp.c, inp.addrbob, inp.token]] ≠ 0
   nullifier_didnt_exist: m .Nullifiers [inp.nullifier crypto] = 0
   r_ne_zero: m .Notes [inp.note_id crypto, 0] ≠ 0
   h_amount: note_amount crypto m (inp.note_id crypto) inp.c = inp.amount
   kbob_private_key: inp.kbob ∈ crypto.PrivateKeys
   amount_ne_zero: inp.amount ≠ 0
+  bob_registered: m .PublicKeys [inp.addrbob] = inp.Kbob crypto
   no_change: ∀ t, ∀ x,
     (t, x) ≠ (.Nullifiers, [inp.nullifier crypto]) →
     m' t x = m t x
@@ -254,7 +255,7 @@ def cancel_note_info
   have ⟨success₀, success₁⟩ := success
   simp only [cancel_note, ne_eq, Bool.decide_and, decide_not, Bool.and_eq_true,
     Bool.not_eq_eq_eq_not, Bool.not_true, decide_eq_false_iff_not, decide_eq_true_eq] at success₀
-  let ⟨subchannel_exists, r_ne_zero, h_amount, kbob_private_key, amount_ne_zero⟩ := success₀
+  let ⟨subchannel_exists, r_ne_zero, h_amount, kbob_private_key, amount_ne_zero, bob_registered⟩ := success₀
 
   simp [cancel_note, ServerAction.run_all, ServerAction.run] at success₁
   have nullifier_didnt_exist := success₁
@@ -268,6 +269,7 @@ def cancel_note_info
     h_amount := h_amount,
     kbob_private_key := kbob_private_key,
     amount_ne_zero := amount_ne_zero,
+    bob_registered := bob_registered,
     no_change := by
       intro t x h₀
       simp [m', h₀, cancel_note, ServerAction.run_all, ServerAction.run]
