lean/privacy/channels/contiguous.lean
@@ -15,10 +15,10 @@ theorem channel_exists_monotone (crypto: Crypto) (rm: ReachableMemory crypto) (a
   case CreateChannel inp =>
     simp only
     let info := create_channel_info crypto inp rm success
-    obtain ⟨addralice, addrbob, Kbob, h⟩ := h
-    use addralice, addrbob, Kbob
+    obtain ⟨addralice, addrbob, h⟩ := h
+    use addralice, addrbob
     rw [ReachableMemory.add_m, run_action, ←info.h_m']
-    by_cases h₀ : crypto.hash [c, addralice, addrbob, Kbob] = inp.channel_hash crypto
+    by_cases h₀ : crypto.hash [c, addralice, addrbob] = inp.channel_hash crypto
     case pos =>
       simp [h₀, info.memory_diff₂]
     case neg =>
